\documentclass{report}
\usepackage{amsmath}

\begin{document}


    $$S K K = (\lambda x y z.x z (y z)) (\lambda x y.x) (\lambda x y.x) $$
    $$= (\lambda x.\lambda y.\lambda z.x z (y z))(\lambda x.\lambda y.x) (\lambda x.\lambda y.x)$$
    $$\xrightarrow[\beta]{} (\lambda y.\lambda z.(\lambda x.\lambda y.x) z (y z)) (\lambda x.\lambda y.x)$$
    $$\xrightarrow[\beta]{} \lambda z.(\lambda x.\lambda y.x) z ((\lambda x.\lambda y.x) z)$$
    $$\xrightarrow[\beta]{} \lambda z.(\lambda x.\lambda y.x) z \lambda y.z$$
    $$\xrightarrow[\beta]{} \lambda z.(\lambda y.z) \lambda y.z
    \xrightarrow[\beta]{} \lambda z.z = I$$

    $$ ((\lambda a.(\lambda b.b b) (\lambda b.b b)) b
    ((\lambda c.(c\:b)) (\lambda a.a))\xrightarrow[\beta]{}$$
    $$((\lambda b.b)(\lambda b.b))((\lambda c.(c b))(\lambda a.a))\xrightarrow[\beta]{}$$
    $$((\lambda b.b)(\lambda b.b))((\lambda a.a) b)\xrightarrow[\beta]{}(\lambda b.b)(\lambda b.b) b$$
\end{document}
